noc/Router.v
@@ -64,13 +64,46 @@ UBind "r_addr" (USugar (UConstBits (Bits.of_nat addr_sz r_addr2)))
         else if dest < r_addr then
         fail
         else
-        rtile_send(extcall Tile_Out(m0));
-        r0_send(pack(subst(msg, new, |1`d0|))) (* To stop the packet from being processed again*)
+        rtile_send(extcall Tile_Out(m0))
+        (* r0_send(pack(subst(msg, new, |1`d0|)))  *)
+        (* To stop the packet from being processed again *)
     else
     pass ))
     ))
 }}.
   
+Definition _routeend_r (r_addr2: nat) (r0_send r0_receive rtile_send: UInternalFunction reg_t ext_fn_t) 
+(Tile_In Tile_Out : ext_fn_t)
+: uaction reg_t ext_fn_t :=
+  UBind "r_addr" (USugar (UConstBits (Bits.of_nat addr_sz r_addr2)))
+  {{
+
+  let m_input := (extcall Tile_In(#bz)) in
+  let msg := unpack(struct_t basic_flit, m_input) in
+  let new_data := get(msg, new) in
+  let src_p := get(msg, src) in
+  (( if (new_data && src_p == r_addr) then
+  r0_send(m_input)
+  else
+  let m0 := r0_receive() in (*router input policy will be added here*)
+  let msg := unpack(struct_t basic_flit, m0) in
+  let new_data := get(msg, new) in
+  let src_p := get(msg, src) in
+  (( if (src_p != r_addr && new_data) then 
+      let dest := get(msg, dest) in
+      (*r_addr[|2`d0| :+ 2] if not using struct*)
+      if dest > r_addr then
+      fail
+      else if dest < r_addr then
+      r0_send(pack(subst(msg, src, r_addr)))
+      else (*Pass to tile from this block*)
+      rtile_send(extcall Tile_Out(m0))
+      (* r0_send(pack(subst(msg, new, |1`d0|))) *)
+  else
+  pass ))
+  ))
+  }}.
+
 (* Router needs to decide which packet will go first then send the packet*)
 Definition _routecenter_r (r_addr2: nat) (r0_send r1_send r0_receive r1_receive rtile_send: UInternalFunction reg_t ext_fn_t) 
 (Tile_In Tile_Out : ext_fn_t)
@@ -101,8 +134,9 @@ Definition _routecenter_r (r_addr2: nat) (r0_send r1_send r0_receive r1_receive 
       else if dest < r_addr then
       r0_send(pack(subst(msg, src, r_addr)))
       else
-      rtile_send(extcall Tile_Out(m0));
-      r0_send(pack(subst(msg, new, |1`d0|))) (* To stop the packet from being processed again*)
+      rtile_send(extcall Tile_Out(m0))
+      (* r0_send(pack(subst(msg, new, |1`d0|)))  *)
+      (* To stop the packet from being processed again*)
   else
   pass ));
   let msg := unpack(struct_t basic_flit, m1) in
@@ -117,44 +151,15 @@ Definition _routecenter_r (r_addr2: nat) (r0_send r1_send r0_receive r1_receive 
       else if dest < r_addr then
       r0_send(pack(subst(msg, src, r_addr)))
       else
-      rtile_send(extcall Tile_Out(m1));
-      r1_send(pack(subst(msg, new, |1`d0|))) (* To stop the packet from being processed again*)
+      rtile_send(extcall Tile_Out(m1))
+      (* r1_send(pack(subst(msg, new, |1`d0|)))  *)
+      (* To stop the packet from being processed again*)
   else
   pass ))
   ))
   }}.
 
-Definition _routeend_r (r_addr2: nat) (r0_send r0_receive rtile_send: UInternalFunction reg_t ext_fn_t) 
-(Tile_In Tile_Out : ext_fn_t)
-: uaction reg_t ext_fn_t :=
-  UBind "r_addr" (USugar (UConstBits (Bits.of_nat addr_sz r_addr2)))
-  {{
 
-  let m_input := (extcall Tile_In(#bz)) in
-  let msg := unpack(struct_t basic_flit, m_input) in
-  let new_data := get(msg, new) in
-  let src_p := get(msg, src) in
-  (( if (new_data && src_p == r_addr) then
-  r0_send(m_input)
-  else
-  let m0 := r0_receive() in (*router input policy will be added here*)
-  let msg := unpack(struct_t basic_flit, m0) in
-  let new_data := get(msg, new) in
-  let src_p := get(msg, src) in
-  (( if (src_p != r_addr && new_data) then 
-      let dest := get(msg, dest) in
-      (*r_addr[|2`d0| :+ 2] if not using struct*)
-      if dest > r_addr then
-      fail
-      else if dest < r_addr then
-      r0_send(pack(subst(msg, src, r_addr)))
-      else (*Pass to tile from this block*)
-      rtile_send(extcall Tile_Out(m0));
-      r0_send(pack(subst(msg, new, |1`d0|)))
-  else
-  pass ))
-  ))
-  }}.
 
 Definition routecenterfn (n:nat) (r1 r2 r_ack: reg_t) (e1 e2: ext_fn_t): uaction reg_t ext_fn_t :=
   _routecenter_r n (r_send r1) (r_send r2) (r_receive r1) (r_receive r2) (r_send r_ack) e1 e2.
